lib/DownTo: Add an alternative compilation lemma without ghost state

src/Rupicola/Lib/ControlFlow/DownTo.v
@@ -1,15 +1,28 @@
-Require Import Rupicola.Lib.Api.
+Require Import Rupicola.Lib.Core.
+Require Import Rupicola.Lib.Notations.
+Require Import Rupicola.Lib.Tactics.
 
 Section Gallina.
-  Definition downto'
-             {state} init start count (step:state->nat->state) : state :=
-    fold_left step (rev (skipn start (seq 0 count))) init.
-  Definition downto
-             {state} init count (step:state->nat->state) : state :=
-    downto' init 0 count step.
+  Context {A: Type}.
+  Implicit Type a : A.
+  Implicit Type step : A -> nat -> A.
+
+  Definition downto' a0 start count step : A :=
+    fold_left step (rev (skipn start (seq 0 count))) a0.
+
+  Definition downto a0 count step : A :=
+    downto' a0 0 count step.
+
+  Open Scope nat_scope.
+
+  Lemma downto'_step start count step a0 :
+    0 < start <= count ->
+    step (downto' a0 start count step) (start - 1) =
+    downto' a0 (start - 1) count step.
+  Proof. cbv [downto']; apply fold_left_skipn_seq. Qed.
 End Gallina.
 
-Section Compile.
+Section Compilation.
   Context {width: Z} {BW: Bitwidth width} {word: word.word width} {mem: map.map word Byte.byte}.
   Context {locals: map.map String.string word}.
   Context {env: map.map String.string (list String.string * list String.string * Syntax.cmd)}.
@@ -20,36 +33,7 @@ Section Compile.
   Context {ext_spec_ok : Semantics.ext_spec.ok ext_spec}.
   Implicit Types (x : word).
 
-  Lemma downto'_step {A} i count (step :A -> _) init :
-    0 < i <= count ->
-    step (downto' init i count step) (i-1) = downto' init (i-1) count step.
-  Proof.
-    cbv [downto']; apply fold_left_skipn_seq.
-  Qed.
-
-  (* helper definition *)
-  Definition downto'_dependent
-             {A B} initA initB start count
-             (stepA : A -> nat -> A) (stepB : A -> B -> nat -> B) :=
-    fold_left_dependent stepA stepB
-                        (rev (skipn start (seq 0 count))) initA initB.
-
-  Lemma downto'_dependent_fst {A B} initA initB stepA stepB i count :
-      fst (@downto'_dependent A B initA initB i count stepA stepB) =
-      downto' initA i count stepA.
-  Proof. apply fold_left_dependent_fst. Qed.
-
-  Lemma downto'_dependent_step
-        {A B} i count stepA stepB (initA : A) (initB : B) :
-    0 < i <= count ->
-    (fun ab c =>
-       (stepA (fst ab) c, stepB (fst ab) (snd ab) c))
-      (downto'_dependent initA initB i count stepA stepB) (i-1)
-    = downto'_dependent initA initB (i-1) count stepA stepB.
-  Proof. apply fold_left_skipn_seq. Qed.
-
-  (* helper lemma for subtracting one from the loop counter -- code does it with
-     words, but proofs want nat *)
+  (* helper lemma for subtracting one from the loop counter *)
   Lemma word_to_nat_sub_1 x n :
     (0 < word.unsigned x)%Z ->
     word.unsigned x = Z.of_nat n ->
@@ -69,18 +53,180 @@ Section Compile.
     x = word.of_Z 0.
   Proof.
     intros. pose proof (word.unsigned_range x).
-    rewrite <-(word.of_Z_unsigned x).
+    rewrite <- (word.of_Z_unsigned x).
     assert (n = 0) by lia; subst.
     change (Z.of_nat 0) with 0%Z in *.
     congruence.
   Qed.
+
+  Lemma compile_downto : forall {tr mem locals functions} {A} (a0: A) count step,
+      let v := downto a0 count step in
+      forall {P} {pred: P v -> predicate} {k: nlet_eq_k P v} {k_impl step_impl}
+        wcount
+        (loop_pred : nat -> A -> predicate) (* loop invariant *)
+        i_var vars,
+
+        loop_pred count a0 tr mem (map.remove locals i_var) ->
+
+        map.get locals i_var = Some wcount ->
+        word.unsigned wcount = Z.of_nat count ->
+        0 < count -> (* FIXME unused *)
+
+        (let v := v in
+         (* loop iteration case *)
+         forall tr l m st i wi,
+           let inv' v tr' mem' locals :=
+               map.get locals i_var = Some wi /\
+               loop_pred i v tr' mem' (map.remove locals i_var) in
+           loop_pred (S i) st tr m (map.remove l i_var) ->
+           word.unsigned wi = Z.of_nat i ->
+           i < count ->
+           <{ Trace := tr;
+              Memory := m;
+              Locals := map.put l i_var wi;
+              Functions := functions }>
+           step_impl
+           <{ inv' (step st i)}>) ->
+        (let v := v in
+         (* continuation *)
+         forall tr l m,
+           loop_pred 0 v tr m (map.remove l i_var) ->
+           map.get l i_var = Some (word.of_Z 0) ->
+           <{ Trace := tr;
+              Memory := m;
+              Locals := l;
+              Functions := functions }>
+           k_impl
+           <{ pred (k v eq_refl) }>) ->
+        (* while (i = n; 0 < i; pass)
+        { i--; step i } *)
+        <{ Trace := tr;
+           Memory := mem;
+           Locals := locals;
+           Functions := functions }>
+        cmd.seq
+          (cmd.while (expr.op bopname.ltu (expr.literal 0) (expr.var i_var))
+                     (cmd.seq (cmd.set i_var (expr.op bopname.sub (expr.var i_var) (expr.literal 1)))
+                              step_impl))
+          k_impl
+        <{ pred (nlet_eq vars v k) }>.
+  Proof.
+    repeat straightline.
+
+    (* handle while *)
+    WeakestPrecondition.unfold1_cmd_goal;
+  (cbv beta match delta [WeakestPrecondition.cmd_body]).
+    exists nat, lt.
+    exists (fun i t m l =>
+         let st :=
+             downto' a0 i count step in
+         loop_pred i st t m (map.remove l i_var)
+         /\ i <= count
+         /\ (exists wi,
+               word.unsigned wi = Z.of_nat i
+               /\ map.get l i_var = Some wi)).
+    ssplit; eauto using lt_wf; [ | ].
+
+    { cbv zeta. subst.
+      cbv [downto'].
+      exists count; ssplit; [ | | exists wcount];
+        repeat match goal with
+               | _ => rewrite skipn_all2 by (rewrite seq_length; lia)
+               | _ => progress subst_lets_in_goal
+               | _ => progress cbn [rev fold_left]
+               | _ => solve [eauto]
+               end. }
+
+    { intros. cleanup; subst.
+      repeat straightline'.
+      lazymatch goal with x := context [word.ltu] |- _ => subst x end.
+      rewrite word.unsigned_ltu, word.unsigned_of_Z_0.
+      match goal with
+      | H1 : ?y = Z.of_nat ?x, H2 : 0 < ?x |- _ =>
+        assert (0 < y)%Z by lia
+      end.
+      destruct_one_match;
+        rewrite ?word.unsigned_of_Z_0, ?word.unsigned_of_Z_1;
+        ssplit; try lia; [ | ].
+      { repeat straightline'.
+        subst_lets_in_goal.
+        lazymatch goal with
+        | Hcmd:context [ WeakestPrecondition.cmd _ ?impl ],
+               Hinv : context [loop_pred _ ?st],
+                      Hi : word.unsigned ?wi = Z.of_nat ?i
+          |- WeakestPrecondition.cmd
+              _ ?impl ?tr ?mem
+              (map.put ?locals ?i_var (word.sub ?wi (word.of_Z 1)))
+              ?post =>
+          specialize (Hcmd tr locals mem st (i-1) (word.sub wi (word.of_Z 1)));
+            replace (S (i-1)) with i in Hcmd by lia;
+            unshelve epose proof (Hcmd _ _ _); clear Hcmd
+        end;
+          [ eauto using word_to_nat_sub_1; lia .. | ].
+        use_hyp_with_matching_cmd; [ ].
+        cbv [postcondition_cmd] in *; sepsimpl; cleanup; subst.
+        repeat match goal with
+               | |- exists _, _ => eexists; ssplit
+               | _ => erewrite <- downto'_step;
+                       [ cbn [fst snd]; ecancel_assumption | ];
+                       lia
+               | _ => lia
+               | _ => solve [eauto using word_to_nat_sub_1]
+               end. }
+      { repeat straightline'.
+        match goal with
+        | H : (word.unsigned ?x <= 0)%Z |- _ =>
+          eapply word_to_nat_0 in H; [ | solve [eauto] .. ]; subst
+        end.
+        match goal with
+          H : word.unsigned (word.of_Z 0) = Z.of_nat ?n |- _ =>
+          assert (n = 0) by (rewrite word.unsigned_of_Z_0 in H; lia)
+        end; subst.
+        use_hyp_with_matching_cmd; subst_lets_in_goal; eauto. } }
+  Qed.
+End Compilation.
+
+Section GhostCompilation.
+  Context {width: Z} {BW: Bitwidth width} {word: word.word width} {mem: map.map word Byte.byte}.
+  Context {locals: map.map String.string word}.
+  Context {env: map.map String.string (list String.string * list String.string * Syntax.cmd)}.
+  Context {ext_spec: bedrock2.Semantics.ExtSpec}.
+  Context {word_ok : word.ok word} {mem_ok : map.ok mem}.
+  Context {locals_ok : map.ok locals}.
+  Context {env_ok : map.ok env}.
+  Context {ext_spec_ok : Semantics.ext_spec.ok ext_spec}.
+  Implicit Types (x : word).
+
+  (* helper definition *)
+  Definition downto'_dependent
+             {A B} initA initB start count
+             (stepA : A -> nat -> A) (stepB : A -> B -> nat -> B) :=
+    fold_left_dependent stepA stepB
+                        (rev (skipn start (seq 0 count))) initA initB.
+
+  Lemma downto'_dependent_fst {A B} initA initB stepA stepB i count :
+      fst (@downto'_dependent A B initA initB i count stepA stepB) =
+      downto' initA i count stepA.
+  Proof. apply fold_left_dependent_fst. Qed.
+
+  Open Scope nat_scope.
+
+  Lemma downto'_dependent_step
+        {A B} i count stepA stepB (initA : A) (initB : B) :
+    0 < i <= count ->
+    (fun ab c =>
+       (stepA (fst ab) c, stepB (fst ab) (snd ab) c))
+      (downto'_dependent initA initB i count stepA stepB) (i-1)
+    = downto'_dependent initA initB (i-1) count stepA stepB.
+  Proof. apply fold_left_skipn_seq. Qed.
 
   (* In this lemma, state refers to the accumulator type for the Gallina downto
      loop, and ghost_state is any extra information that locals/memory invariants
      need access to. *)
   (* FIXME Do we actually need ghost state? *)
   (* TODO: consider taking in range of count instead of providing word? *)
-  Lemma compile_downto : forall {tr mem locals functions} {state} (init : state) count step,
+  Lemma compile_downto_with_ghost_state :
+    forall {tr mem locals functions} {state} (init : state) count step,
     let v := downto init count step in
     forall {P} {pred: P v -> predicate} {k: nlet_eq_k P v} {k_impl step_impl}
       wcount {ghost_state} (ginit : ghost_state)
@@ -211,4 +357,4 @@ Section Compile.
         end; subst.
         use_hyp_with_matching_cmd; subst_lets_in_goal; eauto. } }
   Qed.
-End Compile.
+End GhostCompilation.
